\section{Straight-line path following in the horizontal plane}
\subsection{}
From (2.25) we have: 
\begin{equation}
	\dot{\mathbf{p}}^b_{nb} = \mathbf{R}(\mathbf{\Theta_{nb}}) \mathbf{v}^b_{nb}
\end{equation}

Then: 
\begin{align*}
	\dot{x} &= u \cos(\psi) \cos (\theta) + v [\cos (\psi) \sin( \theta) \sin (\phi) - \sin (\psi) \cos (\theta)] \\
	&+ w [\sin (\psi) \sin (\phi) + \cos (\psi) \cos (\phi) \sin(\theta)] \\
	&= u \cos(\psi) * 1 + v [\cos (\psi) * 0 * 0 - \sin (\psi) * 1] + w [\sin (\psi) * 0 + \cos (\psi) * 1 * 0] \\
	&= u \cos(\psi) - v \sin(\psi) \\
	\dot{y} &= u \sin (\psi) \cos (\theta) 
	+ v [\cos (\psi) \cos (\phi) + \sin (\phi) \sin (\theta) \sin (\psi)] \\
	&+ w [\sin (\theta) \sin (\psi) \cos (\phi) + \cos(\psi) \sin(\phi)] \\ 
	&= u \sin (\psi) * 1
	+ v [\cos (\psi) * 1 + \sin (\phi) * 0 * 0] 
	+ w [0 * \sin (\psi) * 1 + \cos(\psi) * 0] \\ 
	&= u \sin (\psi) + v \cos (\psi) 
\end{align*}
Using: 
\begin{align}
	\sin (\arctan (x)) &= \frac{x}{1 + x^2} \\
	\cos (\arctan (x)) &= \frac{1}{1 + x^2} \\ 
	U &= \sqrt{u^2 + v^2} \\ 
	\beta &= \arctan(\frac{v}{u}) \\
	\chi &= \psi + \beta 
\end{align}

We have: 
\begin{align*}
	\dot{x} &= u \cos(\psi) - v \sin(\psi) 
	= \sqrt{u^2 + v^2} [\cos (\psi) \frac{u}{\sqrt{u^2 + v^2}} 
	- \sin (\psi) \frac{v}{\sqrt{u^2 + v^2}}] \\
	&= U [\cos (\psi) \frac{1}{\sqrt{1 + \frac{v^2}{u^2}}} 
	- \sin (\psi) \frac{\frac{v}{u}}{\sqrt{1 + \frac{v^2}{u^2}}}] \\ 
	&= U [\cos (\psi) \cos(\arctan(\frac{v}{u})) 
	- \sin (\psi) \sin(\arctan(\frac{v}{u}))] 
	= U [\cos (\psi) \cos(\beta)) - \sin (\psi) \sin(\beta))] \\ 
	&= U \cos(\psi + \beta) = U \cos(\chi) \\
	\dot{y} &= u \sin (\psi) + v \cos (\psi) 
	= \sqrt{u^2 + v^2} [\sin (\psi) \frac{u}{\sqrt{u^2 + v^2}}
	+ \cos (\psi) \frac{v}{\sqrt{u^2 + v^2}}] \\
	&= U [\sin (\psi) \frac{1}{\sqrt{1 + \frac{v^2}{u^2}}} 
	+ \cos (\psi) \frac{\frac{v}{u}}{\sqrt{1 + \frac{v^2}{u^2}}}] 
	= U [\sin (\psi) \cos (\arctan(\frac{v}{u}))
	+ \cos (\psi) \sin (\arctan(\frac{v}{u}))] \\
	&= U \sin(\psi + \arctan (\frac{v}{u})) 
	= U \sin(\psi + \beta) 
	= U \sin(\chi)
\end{align*}

\subsection{}
\begin{align}
	\dot{x} &= U \cos (\psi + \beta) \\
	\dot{y} &= U \sin (\psi + \beta) 
\end{align}
With $\beta$ small (and a disturbance) and $\psi$ also small. Then (12) can be seen from Taylor expansion of the sine and cosine functions for small values, with $\dot{x} = U$ and $\dot{y} = U \psi$. 

As the vessel is following a straight line in the horizontal plane, and the assumtions above hold, it is clear that the only part of the cross-track error, $e(t) = -[x(t) - x_k]\sin(\alpha_k) + [y(t) - y_k]\cos(\alpha_k)$, which will affect it is $y$, such that we can give $e(t) = y$. 

\subsection{}
Transfer functions can be written as
\begin{equation}
	H(s) = \frac{a_n s^n + ... + a_1 s + a_0}{b_m s^m + ... + b_1 s + b_0}
\end{equation}

The Nomoto model can be written as
\begin{equation}
\label{eq:nomoto}
	\begin{aligned}
		T \dot{r} + r &= K \delta + b \\
		\dot{\psi} &= r
	\end{aligned}
\end{equation}

Then we can find the transfer functions of \eqref{eq:nomoto} as: 
\begin{align*}
	T s^2 \psi(s) + s \psi(s) &= K \delta(s) + b(s) \\
	s(T s + 1) \frac{s}{U} y(s) &= K \delta(s) + b(s) \\
	y(s) &= \frac{K U}{s^2 (T s + 1)} \delta(s) + \frac{U}{s^2 (T s + 1)} b(s) \\ 
	h_1(s) &= \frac{K U}{s^2 (T s + 1)} \\
	h_2(s) &= \frac{U}{s^2 (T s + 1)}
\end{align*}

The reason we'd like to use the integral term is to remove the bias. The integral can then essentially sum up the bias over time, so that it would be removed. This, however, introduces another integrator into the system, and as we can see above, there are already more integrators there. Therefore, a derivative term is needed to stabilize the system. 

\subsection{}
Answer Problem 2.4 here.  References can be placed in the "bibliography.bib" and referred to as \cite{Fossen2011} and \cite{Fjellstad1994857}. The PID-controller is
\begin{equation}
	\delta = -k_p y - k_d \dot{y} - k_i \int y
\end{equation}
